fixed bug with order typeclass, added example that allocates and uses invariant

src/case_study/examples.v
@@ -6,6 +6,7 @@ From nextgen.case_study Require Export stack_lang stack_transform.
 From iris.proofmode Require Import tactics.
 From stdpp Require Import fin_maps.
 
+From nextgen.lib Require Import invariants.
 From nextgen.case_study Require Import rules_unary stack_lang_notation.
 
 Set Default Proof Using "Type".
@@ -37,10 +38,13 @@ Section examples.
     let: "g" := λ: global, "<>", "f'", "f'" () in
     let: "f" := λ: global, "<>", "<>", let: "x" := sref 42 in "g" (λ: local 0, "<>", "<>", !"x") in
     "f" ().
-    
   
   Definition stuck_example : expr :=
     ! ((λ: global, "<>", "<>", sref 42) ()).
+
+  Definition example4 g : expr :=
+    let: "f" := λ: global, "k", "g", let: "x" := sref 42 in "g" ⟪"x","k"⟫ ;; !"x" in
+    "f" g.
 
 End examples.
 
@@ -121,9 +125,75 @@ Section stack_lang_examples.
     (* STUCK! the points-to for l gets lost, its lifetime is not less than 1 *)
   Abort.
 
+  Definition logN : namespace := nroot .@ "logN".
   
-  
-
+  Lemma example4_spec (e : expr) :
+    (forall v, expr_subst "f" v e = e) -> (* e does not contain free f *)
+    (∀ (j : nat) v1 v2 K', {{{ [size] j
+                      ∗ (∃ (i : nat) K (off : Z), ⌜(off <= 0)%Z⌝ ∧ ⌜shift_expr v2 (-1) = Cont off K⌝ ∧ ⌜(i = j + 1 - (Z.abs_nat off))⌝ ∧
+                                      (∀ v', (∃ n, ⌜v' = Nat n⌝) → [size] i -∗
+                                      ⚡={Ω <- (lifetime_stack i)}=> WP fill K (i,v') {{ λ v, ∃ n, ⌜v.2 = NatV n⌝ }}))
+                      ∗ (∃ i l (off : Z), ⌜(off <= 0)%Z⌝ ∧ ⌜shift_expr v1 (-1) = Loc (local off) l⌝ ∧ ⌜(i = j - (Z.abs_nat off))⌝ ∧
+                                      inv (logN .@ l) (lifetime_stack i) (∃ v, i @@ l ↦ v ∗ ∃ m, ⌜v = NatV m⌝))
+                      ∗ (∀ v', (∃ n, ⌜v' = Nat n⌝) → [size] j -∗
+                        ⚡={Ω <- (lifetime_stack j)}=> WP fill K' (j,v') {{ λ v, ∃ n, ⌜v.2 = NatV n⌝ }}) }}}
+                  fill K' ((j, (λ: global, "k", "x", e) ⟪ v1, v2 ⟫))
+                  {{{ v, RET v; ∃ n, ⌜v.2 = NatV n⌝ }}}) ⊢
+    {{{ [size] 0 }}} (0,example4 (λ: global, "k", "x", e)) {{{ v, RET v; ∃ n, ⌜v.2 = NatV n⌝ }}}.
+  Proof.
+    iIntros (Hfree) "#Hadv_spec".
+    iModIntro. iIntros (Φ) "Hsize #HΦ /=". rewrite /example4. prepare_ctx.
+    iApply wp_LetIn. iIntros "!>". simpl subst'.
+    iApply wp_call_global;[eauto|iFrame]. iIntros "!> Hsize". prepare_ctx.
+    iApply wp_stack_alloc;[lia|repeat constructor|iFrame]. iIntros "!>" (l) "[Hsize Hl] /=". prepare_ctx.
+    iApply wp_LetIn. iIntros "!> /=".
+    prepare_ctx. rewrite Hfree. iApply fupd_wp.
+    iMod (@inv_alloc _ _ _ _ locality_lifetime_pick _ (logN .@ l) _
+            (lifetime_stack 0) (∃ v, 0 @@ l ↦ v ∗ ∃ m, ⌜v = NatV m⌝) with "[Hl]") as "#Hinv".
+    { iSplitR;[|eauto]. iClear "#".
+      iModIntro. iIntros (c' Hle) "Hl". iDestruct "Hl" as (v) "[Hl Hcond]".
+      iDestruct "Hcond" as (m) "->". inversion Hle;subst.
+      - rewrite -next_state_eq. iModIntro. eauto.
+      - iDestruct (stack_stack_pop_intro _ _ _ _ f2 with "Hl") as "Hl";[auto|].
+        rewrite -next_state_eq. iModIntro. eauto. }
+    iApply ("Hadv_spec" with "[-] [//]"). iFrame.
+    iSplitR;[|iSplitR].
+    - (* the unknown function returns to the first caller *)
+      iExists 0,[],(-2)%Z.
+      iSplit;[iPureIntro;lia|].
+      iSplit;[auto|].
+      iSplit;[iPureIntro;lia|].
+      iIntros (v' Hv') "Hsize".
+      iClear "Hinv Hadv_spec". iModIntro.
+      destruct Hv' as [? ->]. simpl. iApply wp_value;eauto.
+    - (* invariant for the stack variable parameter *)
+      iExists 0,l,(-1)%Z.
+      iSplit;[iPureIntro;lia|].
+      iSplit;[auto|].
+      iSplit;[iPureIntro;lia|].
+      iFrame "Hinv".
+    - (* the unknown function returns normally to the caller *)
+      iIntros (v' [? ->]) "Hsize".
+      iDestruct (next_state_stack_inv_intro _ _ 1 with "Hinv") as "Hinv'";[lia|].
+      iClear "Hinv Hadv_spec". iRename "Hinv'" into "Hinv".
+      iModIntro. iSimpl.  prepare_ctx.
+      iApply wp_LetIn. iNext. iSimpl. prepare_ctx.
+      iApply (wp_atomic_under_ectx _ (⊤ ∖ ↑logN.@l));eauto.
+      { apply is_atomic_correct;eauto. }
+      { apply is_atomic_sub_values;eauto. }
+      { apply is_atomic_normal;eauto. }
+      { unfold SameGeneration. by cbn. }
+      iMod (inv_acc with "Hinv") as "[>Hl Hcls]";[set_solver|].
+      iDestruct "Hl" as (v) "[Hl %Heq]". destruct Heq as [? ->].
+      iModIntro. prepare_ctx. iApply wp_stack_load;[repeat constructor;lia|].
+      iFrame. iIntros "!> [Hsize Hl] /=".
+      iApply wp_value. iMod ("Hcls" with "[Hl]") as "_";[eauto|].
+      iModIntro. prepare_ctx.
+      iApply wp_return;[lia|lia|]. iFrame.
+      iIntros "!> Hsize". iClear "Hinv". iModIntro.
+      simpl. iApply wp_value. eauto.
+  Qed.
+      
 End stack_lang_examples.
 
 
